Add Read() (not yet verifying)

TestModels/dafny-dependencies/StandardLibrary/src/Streams.dfy
@@ -3,7 +3,6 @@
  *  SPDX-License-Identifier: MIT
  *******************************************************************************/
 
-// TODO: Relocate under Actions/ instead, I don't think Streams has to be a separate library?
 module {:options "--function-syntax:4"} Std.Streams {
 
   import opened Wrappers
@@ -18,7 +17,7 @@ module {:options "--function-syntax:4"} Std.Streams {
   //
   // Allows for streams that can only be read once,
   // but see RewindableDataStream for a more specific trait
-  // that requires the ability to replay the enumeration,
+  // that requires the ability to replay the data,
   // or seek to an arbitrary position (although this may take linear time).
   // That requirement is not in this trait
   // because there are lots of ways to implement a stream
@@ -31,50 +30,51 @@ module {:options "--function-syntax:4"} Std.Streams {
   @AssumeCrossModuleTermination
   trait DataStream<T, E> extends Producer<Result<seq<T>, E>> {
 
-    ghost const data: seq<T>
-
     // The total length of all produced batches
-    function ContentLength(): (res: Option<uint64>)
-      requires Valid()
-      reads this, Repr
-
-    ghost predicate ValidOutputs(outputs: seq<Option<Result<seq<T>, E>>>)
-      requires Seq.Partitioned(outputs, IsSome)
-      ensures ValidOutputs(outputs) ==> ValidDataSoFar(outputs)
-      decreases Repr
-
-    ghost predicate ValidDataSoFar(outputs: seq<Option<Result<seq<T>, E>>>)
-      requires Partitioned(outputs, IsSome)
-    {
-      var produced := ProducedOf(outputs);
-      && var dataSoFar := DataSoFar(produced);
-      && (dataSoFar.Some? ==> 
-        && dataSoFar.value <= data
-        && (!Seq.All(outputs, IsSome) ==> dataSoFar.value == data))
-    }
-
-    ghost function DataSoFar(produced: seq<Result<seq<T>, E>>): Option<seq<T>>
-    {
-      if exists o <- produced :: o.Failure? then
-        None
-      else
-        Some(Flatten(MapPartialFunction((o: Result<seq<T>, E>) requires o.Success? => o.value, produced)))
-    }
-  }
-
-  trait RewindableDataStream<T, E> extends DataStream<T, E> {
+    const contentLength: Option<uint64>
 
     ghost predicate Valid()
       reads this, Repr
       ensures Valid() ==> this in Repr
       ensures Valid() ==> ValidHistory(history)
-      ensures Valid() ==> |data| <= UINT64_MAX as int
       decreases Repr, 0
 
-    function ContentLength(): (res: Option<uint64>)
-      requires Valid()
-      reads this, Repr
-      ensures res == Some(|data| as uint64)
+    ghost predicate ValidOutputs(outputs: seq<Option<Result<seq<T>, E>>>)
+      requires Seq.Partitioned(outputs, IsSome)
+      ensures ValidOutputs(outputs) && contentLength.Some? ==> ValidDataSoFar(outputs, contentLength.value as int)
+      decreases Repr
+
+    method Read(max: uint64) returns (r: Option<Result<seq<T>, E>>)
+      requires Requires(())
+      reads Reads(())
+      modifies Modifies(())
+      decreases Decreases(())
+      ensures Ensures((), r)
+      ensures 0 < max ==> RemainingDecreasedBy(r)
+      ensures r.Some? && r.value.Success? ==> |r.value.value| <= max as int
+  }
+
+  ghost predicate ValidDataSoFar<T, E>(outputs: seq<Option<Result<seq<T>, E>>>, length: int)
+    requires Partitioned(outputs, IsSome)
+  {
+    var produced := ProducedOf(outputs);
+    && var dataSoFar := DataSoFar(produced);
+    && (dataSoFar.Some? ==> 
+      && |dataSoFar.value| <= length
+      && (!Seq.All(outputs, IsSome) ==> |dataSoFar.value| == length))
+  }
+
+  ghost function DataSoFar<T, E>(produced: seq<Result<seq<T>, E>>): Option<seq<T>>
+  {
+    if exists o <- produced :: o.Failure? then
+      None
+    else
+      Some(Flatten(MapPartialFunction((o: Result<seq<T>, E>) requires o.Success? => o.value, produced)))
+  }
+    
+  trait RewindableDataStream<T, E> extends DataStream<T, E> {
+
+    ghost const data: seq<T>
 
     function Position(): (res: uint64)
       requires Valid()
@@ -89,13 +89,37 @@ module {:options "--function-syntax:4"} Std.Streams {
       ensures Position() == newPosition
   }
 
+  ghost predicate ValidDataLengthSoFar<T>(outputs: seq<Option<seq<T>>>, length: int)
+    requires Partitioned(outputs, IsSome)
+  {
+    var dataSoFar := Flatten(ProducedOf(outputs));
+    && |dataSoFar| <= length
+    && (!Seq.All(outputs, IsSome) ==> |dataSoFar| == length)
+  }
+
+  trait ProducesTotalLengthProof<T> {
+
+    const producer: Producer<seq<T>>
+    const length: int
+
+    lemma ProducesTotalLength(history: seq<((), Option<seq<T>>)>)
+      requires producer.ValidHistory(history)
+      ensures ValidDataLengthSoFar(OutputsOf(history), length)
+  }
+
   /*
    * Wraps an Producer up as a non-rewindable DataStream that cannot error.
+   * It implements Read() using Next(), and buffers extra data
+   * as needed.
    */
   class ProducerDataStream<T> extends DataStream<T, ()> {
 
     const wrapped: Producer<seq<T>>
     const length: uint64
+    var buffer: seq<T>
+
+    ghost const producesTotalLengthProof: ProducesTotalLengthProof<T>
+    ghost const maxWrappedRemaining: TerminationMetric
 
     ghost predicate Valid()
       reads this, Repr
@@ -106,14 +130,17 @@ module {:options "--function-syntax:4"} Std.Streams {
       && this in Repr
       && ValidComponent(wrapped)
       && ValidHistory(history)
+      && producesTotalLengthProof.producer == wrapped
+      && producesTotalLengthProof.length == length as int
+      && |buffer| <= length as int
     }
 
     ghost predicate ValidOutputs(outputs: seq<Option<Result<seq<T>, ()>>>)
       requires Seq.Partitioned(outputs, IsSome)
-      ensures ValidOutputs(outputs) ==> ValidDataSoFar(outputs)
+      ensures ValidOutputs(outputs) && contentLength.Some? ==> ValidDataSoFar(outputs, contentLength.value as int)
       decreases Repr
     {
-      ValidDataSoFar(outputs)
+      contentLength.Some? ==> ValidDataSoFar(outputs, contentLength.value as int)
     }
 
     ghost function RemainingMetric(): TerminationMetric 
@@ -121,27 +148,24 @@ module {:options "--function-syntax:4"} Std.Streams {
       reads this, Repr
       decreases Repr, 3
     {
-      TMSucc(wrapped.RemainingMetric())
+      TMTuple(maxWrappedRemaining, wrapped.RemainingMetric(), TMNat(|buffer|))
     }
 
-    constructor(wrapped: Producer<seq<T>>, length: uint64)
+    constructor(wrapped: Producer<seq<T>>, length: uint64, ghost producesTotalLengthProof: ProducesTotalLengthProof<T>)
       requires wrapped.Valid()
       requires wrapped.history == []
+      requires producesTotalLengthProof.producer == wrapped
+      requires producesTotalLengthProof.length == length as int
       ensures Valid()
       ensures fresh(Repr - wrapped.Repr)
     {
       this.wrapped := wrapped;
       this.length := length;
+      this.buffer := [];
 
       this.history := [];
       this.Repr := {this} + wrapped.Repr;
-    }
-
-    function ContentLength(): (res: Option<uint64>)
-      requires Valid()
-      reads this, Repr
-    {
-      Some(length)
+      this.producesTotalLengthProof := producesTotalLengthProof;
     }
 
     method Invoke(i: ()) returns (r: Option<Result<seq<T>, ()>>)
@@ -165,15 +189,61 @@ module {:options "--function-syntax:4"} Std.Streams {
       // TODO: work to do
       assume {:axiom} Valid();
       if r.Some? {
-        old(RemainingMetric()).SuccDecreasesToSucc(RemainingMetric());
+        old(RemainingMetric()).TupleDecreasesToTuple(RemainingMetric());
       } else {
-        old(RemainingMetric()).SuccNonIncreasesToSucc(RemainingMetric());
+        old(RemainingMetric()).TupleNonIncreasesToTuple(RemainingMetric());
       }
+    }
+
+    method Read(max: uint64) returns (r: Option<Result<seq<T>, ()>>)
+      requires Requires(())
+      reads Reads(())
+      modifies Modifies(())
+      decreases Decreases(())
+      ensures Ensures((), r)
+      ensures 0 < max ==> RemainingDecreasedBy(r)
+      ensures r.Some? && r.value.Success? ==> |r.value.value| <= max as int
+    {
+      assert Requires(());
+
+      assert Valid();
+      var next;
+      if 0 < |buffer| {
+        next := Some(buffer);
+        buffer := [];
+      } else {
+        next := wrapped.Next();
+      }
+      assert next.Some? ==> |next.value| <= length as int;
+
+      if next.None? {
+        r := None;
+
+        OutputsPartitionedAfterOutputtingNone();
+        ProduceNone();
+      } else {
+        var size := if max <= |next.value| as uint64 then max else |next.value| as uint64;
+        var value := Success(next.value[..size]);
+        r := Some(value);
+        buffer := next.value[size..];
+
+        OutputsPartitionedAfterOutputtingSome(value);
+        ProduceSome(value);
+      }
+      
+      if 0 < max {
+        if r.Some? {
+          old(RemainingMetric()).TupleDecreasesToTuple(RemainingMetric());
+        } else {
+          old(RemainingMetric()).TupleNonIncreasesToTuple(RemainingMetric());
+        }
+      }
+      assert 0 < max ==> RemainingDecreasedBy(r);
     }
   }
 
   /*
-   * Rewindable stream of a sequence with a configured chunk size.
+   * Rewindable stream of a sequence with a configured default chunk size.
    */
   class SeqDataStream<T> extends RewindableDataStream<T, ()> {
 
@@ -192,16 +262,18 @@ module {:options "--function-syntax:4"} Std.Streams {
       && ValidHistory(history)
       && s == data
       && |s| <= UINT64_MAX as int
+      && contentLength == Some(|s| as uint64)
       && position as int <= |s|
       && 0 < chunkSize
     }
 
     ghost predicate ValidOutputs(outputs: seq<Option<Result<seq<T>, ()>>>)
       requires Seq.Partitioned(outputs, IsSome)
-      ensures ValidOutputs(outputs) ==> ValidDataSoFar(outputs)
+      ensures ValidOutputs(outputs) && contentLength.Some? ==> ValidDataSoFar(outputs, contentLength.value as int)
       decreases Repr
     {
-      ValidDataSoFar(outputs)
+      && contentLength.Some?
+      && ValidDataSoFar(outputs, contentLength.value as int)
     }
 
     ghost function RemainingMetric(): TerminationMetric 
@@ -221,6 +293,7 @@ module {:options "--function-syntax:4"} Std.Streams {
       this.s := s;
       this.position := 0;
       this.chunkSize := chunkSize;
+      this.contentLength := Some(|s| as uint64);
 
       this.history := [];
       this.Repr := {this};
@@ -242,6 +315,7 @@ module {:options "--function-syntax:4"} Std.Streams {
       position
     }
 
+    @ResourceLimit("0")
     method Seek(newPosition: uint64)
       requires Valid()
       requires newPosition as int <= |data|
@@ -261,10 +335,9 @@ module {:options "--function-syntax:4"} Std.Streams {
       var dataSoFar := DataSoFar(produced);
       if outputs == [] {
         assert produced == [];
-        assert (forall o <- produced :: o.Success? ==> 0 < |o.value|);
       } else {
         assert outputs == [Some(Success(s[..position]))];
-        assert produced == [Success(s[..position])];
+        assert produced == [Success(s[..position])] + ProducedOf([]);
         assert MapPartialFunction((o: Result<seq<T>, ()>) requires o.Success? => o.value, produced) == [s[..position]];
         assert Flatten([s[..position]]) == s[..position];
         assert dataSoFar == Some(s[..position]);
@@ -273,30 +346,47 @@ module {:options "--function-syntax:4"} Std.Streams {
 
     method Invoke(t: ()) returns (r: Option<Result<seq<T>, ()>>)
       requires Requires(t)
-      reads Reads(t)
+      reads this, Repr
       modifies Modifies(t)
       decreases Decreases(t), 0
       ensures Ensures(t, r)
       ensures RemainingDecreasedBy(r)
     {
-      assert Requires(t);
+      assert Valid();
+      r := Read(chunkSize);
+    }
+
+    method Read(max: uint64) returns (r: Option<Result<seq<T>, ()>>)
+      requires Requires(())
+      reads this, Repr
+      modifies Modifies(())
+      decreases Decreases(())
+      ensures Ensures((), r)
+      ensures 0 < max ==> RemainingDecreasedBy(r)
+      ensures r.Some? && r.value.Success? ==> |r.value.value| <= max as int
+    {
+      assert Requires(());
 
       assert Valid();
       if position == |s| as uint64 {
         r := None;
+
+        OutputsPartitionedAfterOutputtingNone();
+        ProduceNone();
       } else {
         // Warning: unbounded integers
-        var size := Math.Min(chunkSize as int, |s| - position as int) as uint64;
+        var remaining := |s| as uint64 - position;
+        var size := if max <= remaining then max else remaining;
         var newPosition := position + size;
-        r := Some(Success(s[position..newPosition]));
+        var chunk := Success(s[position..newPosition]);
+        r := Some(chunk);
         position := newPosition;
+
+        OutputsPartitionedAfterOutputtingSome(chunk);
+        ProduceSome(chunk);
       }
-      UpdateHistory(t, r);
 
       reveal TerminationMetric.Ordinal();
-
-      // TODO: Work to do
-      assume {:axiom} Ensures(t, r);
     }
   }
 }
